src/CLI/Analyse_Dispatch.thy
@@ -977,6 +977,7 @@ code_identifier
 | code_module VIMP_Proc_to_CFG \<rightharpoonup> (OCaml) Core
 | code_module Compile_Wellformed \<rightharpoonup> (OCaml) Core
 | code_module Abstract_Domain \<rightharpoonup> (OCaml) Core
+| code_module Backward_Domain \<rightharpoonup> (OCaml) Core
 | code_module Numeric_Ops \<rightharpoonup> (OCaml) Core
 | code_module Exec_St \<rightharpoonup> (OCaml) Core
 | code_module AList \<rightharpoonup> (OCaml) Core
