src/Examples/Sign/Example_Sign_Placement.thy
@@ -1,7 +1,7 @@
 theory Example_Sign_Placement
   imports "Voblint_VIMP.VIMP_Notation" "Voblint_Analysis.Sign_Exec" "Voblint_Exec.Exec_DG_Bridge"
     "Voblint_Exec.Solver_Menu" "Voblint_CFG.CFG_Prune" "Voblint_Core.DG_LTR_Sound"
-    "Voblint_Compile.Compile_Invariants"
+    "Voblint_Compile.Compile_Invariants" Placement_Policy
 begin
 
 hide_const phase.N
